fix a bunch of type errors

examples/scache/AtomicStatus.i.dfy
@@ -9,40 +9,41 @@ module AtomicStatusImpl {
   import opened Ptrs
   import opened AtomicSpec
   import opened LinearMaybe
-  import ReadWriteLockResources
+  import RWLock
 
   const flag_free : uint8 := 0;
   const flag_back : uint8 := 1;
   const flag_write : uint8 := 2;
   const flag_back_write : uint8 := 3;
 
-  type AtomicStatus = Atomic<uint8, ReadWriteLockResources.Q>
+  type AtomicStatus = Atomic<uint8, RWLock.R>
 
-  predicate state_inv(v: uint8, g: ReadWriteLockResources.Q, ptr: Ptr)
+  predicate state_inv(v: uint8, g: RWLock.R, key: RWLock.Key)
   {
-    && g.FlagsField?
-    && g.ptr == ptr
-    && (g.flags == ReadWriteLockResources.Free ==> v == flag_free)
-    && (g.flags == ReadWriteLockResources.Back ==> v == flag_back)
-    && (g.flags == ReadWriteLockResources.Write ==> v == flag_write)
-    && (g.flags == ReadWriteLockResources.Back_PendingWrite ==>
+    && g.Internal?
+    && g.q.FlagsField?
+    && g.q.key == key
+    && (g.q.flags == RWLock.Free ==> v == flag_free)
+    && (g.q.flags == RWLock.Back ==> v == flag_back)
+    && (g.q.flags == RWLock.Write ==> v == flag_write)
+    && (g.q.flags == RWLock.Back_PendingWrite ==>
         v == flag_back_write)
   }
 
-  predicate atomic_status_inv(a: AtomicStatus, ptr: Ptr)
+  predicate atomic_status_inv(a: AtomicStatus, key: RWLock.Key)
   {
-    forall v, g :: atomic_inv(a, v, g) <==> state_inv(v, g, ptr)
+    forall v, g :: atomic_inv(a, v, g) <==> state_inv(v, g, key)
   }
 
   method unsafe_obtain<Q>() returns (linear r: Q)
   method unsafe_dispose<Q>(linear r: Q)
 
-  method try_acquire_writeback(a: AtomicStatus, ptr: Ptr)
-  returns (success: bool, linear m: maybe<ReadWriteLockResources.Q>)
-  requires atomic_status_inv(a, ptr)
+  method try_acquire_writeback(a: AtomicStatus, key: RWLock.Key)
+  returns (success: bool, linear m: maybe<RWLock.R>)
+  requires atomic_status_inv(a, key)
   ensures !success ==> !has(m)
   ensures success ==> has(m)
-      && read(m) == ReadWriteLockResources.BackObtained(ptr)
+      && read(m) == RWLock.Internal(RWLock.BackObtained(key))
   {
     // TODO check if the acquire flag is set
 
@@ -59,7 +60,7 @@ module AtomicStatusImpl {
       var v2 := flag_back;
       var old_v: uint8;
       var new_v: uint8;
-      linear var old_g: ReadWriteLockResources.Q := unsafe_obtain();
+      linear var old_g: RWLock.R := unsafe_obtain();
       assume old_v == v1 ==> new_v == v2 && did_set;
       assume old_v != v1 ==> new_v == old_v && !did_set;
       assume atomic_inv(a, old_v, old_g);
@@ -67,13 +68,13 @@ module AtomicStatusImpl {
       ///// Transfer:
       if did_set {
         linear var res;
-        new_g, res := ReadWriteLockResources.transform_TakeBack(ptr, old_g);
+        new_g, res := RWLock.transform_TakeBack(key, old_g);
         m := give(res);
       } else {
         m := empty();
         new_g := old_g;
       }
-      assert state_inv(new_v, new_g, ptr);
+      assert state_inv(new_v, new_g, key);
       ///// Teardown:
       assert atomic_inv(a, new_v, new_g);
       unsafe_dispose(new_g);
@@ -83,12 +84,12 @@ module AtomicStatusImpl {
     }
   }
 
-  method try_set_write_lock(a: AtomicStatus, ptr: Ptr)
-  returns (success: bool, linear m: maybe<ReadWriteLockResources.Q>)
-  requires atomic_status_inv(a, ptr)
+  method try_set_write_lock(a: AtomicStatus, key: RWLock.Key)
+  returns (success: bool, linear m: maybe<RWLock.R>)
+  requires atomic_status_inv(a, key)
   ensures !success ==> !has(m)
   ensures success ==> has(m)
-      && read(m) == ReadWriteLockResources.WritePendingAwaitBack(ptr)
+      && read(m) == RWLock.Internal(RWLock.WritePendingAwaitBack(key))
   {
     var orig_value := fetch_or(a, flag_write);
 
@@ -97,20 +98,20 @@ module AtomicStatusImpl {
     var v := flag_write;
     var old_v: uint8;
     var new_v: uint8;
-    linear var old_g: ReadWriteLockResources.Q := unsafe_obtain();
+    linear var old_g: RWLock.R := unsafe_obtain();
     assume orig_value == old_v;
     assume new_v == bit_or(old_v, v);
     assume atomic_inv(a, old_v, old_g);
     linear var new_g;
     ///// Transfer:
-    var fl := old_g.flags;
-    if fl == ReadWriteLockResources.Free {
+    var fl := old_g.q.flags;
+    if fl == RWLock.Free {
       linear var r;
-      new_g, r := ReadWriteLockResources.transform_TakeWrite(ptr, old_g);
+      new_g, r := RWLock.transform_TakeWrite(key, old_g);
       m := give(r);
-    } else if fl == ReadWriteLockResources.Back {
+    } else if fl == RWLock.Back {
       linear var r;
-      new_g, r := ReadWriteLockResources.transform_TakeWriteAwaitBack(ptr, old_g);
+      new_g, r := RWLock.transform_TakeWriteAwaitBack(key, old_g);
       m := give(r);
     } else {
       new_g := old_g;
@@ -124,13 +125,13 @@ module AtomicStatusImpl {
     success := bit_and(orig_value, flag_write) == 0;
   }
 
-  method try_check_writeback_isnt_set(a: AtomicStatus, ptr: Ptr,
-      linear m: ReadWriteLockResources.Q)
-  returns (success: bool, linear m': ReadWriteLockResources.Q)
-  requires atomic_status_inv(a, ptr)
-  requires m == ReadWriteLockResources.WritePendingAwaitBack(ptr)
+  method try_check_writeback_isnt_set(a: AtomicStatus, key: RWLock.Key,
+      linear m: RWLock.R)
+  returns (success: bool, linear m': RWLock.R)
+  requires atomic_status_inv(a, key)
+  requires m == RWLock.Internal(RWLock.WritePendingAwaitBack(key))
   ensures !success ==> m' == m
-  ensures success ==> m' == ReadWriteLockResources.WritePending(ptr, 0)
+  ensures success ==> m' == RWLock.Internal(RWLock.WritePending(key, 0))
   {
     var f := atomic_read(a);
 
@@ -138,17 +139,17 @@ module AtomicStatusImpl {
     ///// Setup:
     var old_v: uint8;
     var new_v: uint8;
-    linear var old_g: ReadWriteLockResources.Q := unsafe_obtain();
+    linear var old_g: RWLock.R := unsafe_obtain();
     assume new_v == old_v;
     assume f == old_v;
     assume atomic_inv(a, old_v, old_g);
     linear var new_g;
     ///// Transfer:
-    var fl := old_g.flags;
-    if fl == ReadWriteLockResources.Free
-        || fl == ReadWriteLockResources.Write
+    var fl := old_g.q.flags;
+    if fl == RWLock.Free
+        || fl == RWLock.Write
     {
-      new_g, m' := ReadWriteLockResources.transform_TakeWriteFinishBack(ptr, fl, old_g, m);
+      new_g, m' := RWLock.transform_TakeWriteFinishBack(key, fl, old_g, m);
     } else {
       new_g := old_g;
       m' := m;
