examples/scache/DiskIO.i.dfy
@@ -5,16 +5,17 @@ include "CacheResources.i.dfy"
 module DiskIO {
   import opened Ptrs
   import opened NativeTypes
-  import ReadWriteLockResources
+  import RWLock
   import CacheResources
 
   linear datatype WritebackGhostState = WritebackGhostState(
-      linear q: ReadWriteLockResources.Q,
-      linear cache_entry: CacheResources.R, // TODO should be readonly
-      linear idx: ConstDeref<int>)
+      linear q: RWLock.R,
+      /*readonly*/ linear cache_entry: CacheResources.R,
+      /*readonly*/ linear idx: Deref<int>)
 
   method disk_writeback_async(addr: uint64,
-      ptr: Ptr, linear contents: Ptrs.R<byte>,
+      ptr: Ptr,
+      /*readonly*/ linear contents: Ptrs.ArrayDeref<byte>,
       linear g: WritebackGhostState)
   requires contents.ptr == ptr
   requires |contents.s| == 4096
